ring leader election decentralized monotonic

messageInvariantPrototypes/ringLeaderElection/decentralizedMonotonic/spec.dfy
@@ -5,36 +5,22 @@ module Obligations {
   import opened UtilitiesLibrary
   import opened DistributedSystem
 
-
-  ghost predicate IsLeader(c: Constants, v: Variables, idx: int)
-    requires c.WF()
-    requires v.WF(c)
+ghost predicate IsLeader(c: Constants, h: Hosts, idx: nat) 
+    requires h.WF(c)
     requires c.ValidIdx(idx)
-  {
-    v.Last().hosts[idx].highestHeard == c.hostConstants[idx].hostId
-  }
-
-  ghost predicate Safety(c: Constants, v: Variables) 
-    requires c.WF()
-    requires v.WF(c)
-  {
-    forall idx1, idx2 | 
-      && c.ValidIdx(idx1) 
-      && c.ValidIdx(idx2) 
-      && IsLeader(c, v, idx1)
-      && IsLeader(c, v, idx2)
-      :: idx1 == idx2
-  }
-
-  /***************************************************************************************
-  *                                      Utils                                           *
-  ***************************************************************************************/
-
-  lemma SuccessorPredecessorRelation(n: int, idx: nat) 
-    requires 0 < n
-    requires idx < n
-    ensures Predecessor(n, Successor(n, idx)) == idx
-    ensures Successor(n, Predecessor(n, idx)) == idx
-  {}
-
+{
+    h.hosts[idx].highestHeard == c.hostConstants[idx].hostId
 }
+
+ghost predicate Safety(c: Constants, v: Variables) 
+    requires v.WF(c)
+{
+    forall idx1, idx2 | 
+        && c.ValidIdx(idx1) 
+        && c.ValidIdx(idx2) 
+        && IsLeader(c, v.Last(), idx1)
+        && IsLeader(c, v.Last(), idx2)
+        :: idx1 == idx2
+}
+}
+
